Prove that `compileFn` produces `Proc`s with affine channel usage. (#10)
* WIP prove that compileFn preserves affine channel usage

* Tweaks to AffineChan definition

* More work on compileFn_affine_var_imp_affine_chan

* [claude] Some progress on compileFn_affine_var_imp_atoms_pairwise_disj_io

* Partial progress

* More progress except for compileExpr_outputs_overapprox

* [claude] Finish compileExpr_outputs_overapprox

wavelet-core/lean/Wavelet/Dataflow/AffineChan.lean
@@ -8,11 +8,9 @@ open Semantics
 /-- Each channel name is used at most once. -/
 def AtomicProcs.AffineChan [Arity Op] (aps : AtomicProcs Op χ V) : Prop
   :=
-  (∀ (i : Fin aps.length),
-    aps[i].inputs.Nodup ∧ aps[i].outputs.Nodup) ∧
-  (∀ (i j : Fin aps.length), i ≠ j →
-    aps[i].inputs.Disjoint aps[j].inputs ∧
-    aps[i].outputs.Disjoint aps[j].outputs)
+  (∀ ap ∈ aps, ap.inputs.Nodup ∧ ap.outputs.Nodup) ∧
+  aps.Pairwise (λ ap₁ ap₂ =>
+    ap₁.inputs.Disjoint ap₂.inputs ∧ ap₁.outputs.Disjoint ap₂.outputs)
 
 /-- Each channel name is used at most once. -/
 def Proc.AffineChan [Arity Op] (proc : Proc Op χ V m n) : Prop :=
@@ -34,9 +32,9 @@ def AtomicProc.checkNoDupIO [Arity Op] [DecidableEq χ]
 /-- Helper function to check that no atom has duplicate intputs or outputs. -/
 def AtomicProcs.checkNoDupIO [Arity Op] [DecidableEq χ]
   (aps : AtomicProcs Op χ V) : Except String Unit
-  := (List.finRange aps.length).forM λ i => do
-    aps[i].checkNoDupIO.mapError λ err =>
-      s!"atomic proc {i}: {err}"
+  := aps.forM λ ap => do
+    ap.checkNoDupIO.mapError λ err =>
+      s!"atomic proc has duplicate IO: {err}"
 
 /-- Executable version of `AtomicProcs.AffineChan`. -/
 def AtomicProcs.checkAffineChan [Arity Op] [DecidableEq χ] [Repr χ]
@@ -45,7 +43,7 @@ def AtomicProcs.checkAffineChan [Arity Op] [DecidableEq χ] [Repr χ]
   aps.checkNoDupIO
   (List.finRange aps.length).forM λ i => do
     (List.finRange aps.length).forM λ j => do
-      if i ≠ j then
+      if i < j then
         if ¬ aps[i].inputs.Disjoint aps[j].inputs then
           throw s!"atomic procs {i} and {j} have overlapping inputs"
         if ¬ aps[i].outputs.Disjoint aps[j].outputs then
@@ -87,11 +85,10 @@ theorem AtomicProcs.checkNoDupIO.correct
   [Arity Op] [DecidableEq χ]
   {aps : AtomicProcs Op χ V} :
     aps.checkNoDupIO.isOk ↔
-    ∀ (i : Fin aps.length), aps[i].inputs.Nodup ∧ aps[i].outputs.Nodup
+    ∀ ap ∈ aps, ap.inputs.Nodup ∧ ap.outputs.Nodup
   := by
   simp only [AtomicProcs.checkNoDupIO, List.forM_ok_iff_all_ok]
   simp [← AtomicProc.checkNoDupIO.correct]
-  grind only [List.mem_finRange, =_ List.contains_iff_mem, cases Or]
 
 theorem AtomicProcs.checkAffineChan.correct
   [Arity Op] [DecidableEq χ] [Repr χ]
@@ -107,9 +104,10 @@ theorem AtomicProcs.checkAffineChan.correct
     · apply AtomicProcs.checkNoDupIO.correct.mp
       simp [h₁, Except.isOk, Except.toBool]
     · simp only [forM, List.forM_ok_iff_all_ok] at h
-      intros i j hne
-      specialize h i (List.mem_finRange _) j (List.mem_finRange _)
-      simp [hne] at h
+      simp [List.pairwise_iff_getElem]
+      intros i j hi hj hlt
+      specialize h ⟨i, hi⟩ (List.mem_finRange _) ⟨j, hj⟩ (List.mem_finRange _)
+      simp [hlt] at h
       split at h
       any_goals contradiction
       rename_i h₂
@@ -125,11 +123,12 @@ theorem AtomicProcs.checkAffineChan.correct
       simp [h₁, Except.isOk, Except.toBool] at this
     · simp only [forM, List.forM_ok_iff_all_ok]
       intros i _ j _
-      split; rfl
-      rename_i h₂
-      have := h.2 i j h₂
-      simp at this
-      simp [this, pure, Except.pure, Except.isOk, Except.toBool]
+      split
+      · rename_i h₂
+        have := (List.pairwise_iff_getElem.mp h.2) i j (by simp) (by simp) h₂
+        simp at this
+        simp [this, pure, Except.pure, Except.isOk, Except.toBool]
+      · rfl
 
 theorem Proc.checkAffineChan.correct
   [Arity Op] [DecidableEq χ] [Repr χ]
@@ -198,8 +197,14 @@ theorem Proc.AffineChan.atom_inputs_disjoint
   (hne : i ≠ j) :
     proc.atoms[i].inputs.Disjoint proc.atoms[j].inputs
   := by
-  have ⟨_, _, hatoms, _, _⟩ := haff
-  exact (hatoms.2 i j hne).1
+  if hlt : i < j then
+    have ⟨_, _, hatoms, _, _⟩ := haff
+    exact ((List.pairwise_iff_getElem.mp hatoms.2) i j (by simp) (by simp) hlt).1
+  else
+    have ⟨_, _, hatoms, _, _⟩ := haff
+    have hlt : j < i := by omega
+    have := ((List.pairwise_iff_getElem.mp hatoms.2) j i (by simp) (by simp) hlt).1
+    exact this.symm
 
 theorem Proc.AffineChan.atom_outputs_disjoint
   [Arity Op]
@@ -209,7 +214,24 @@ theorem Proc.AffineChan.atom_outputs_disjoint
   (hne : i ≠ j) :
     proc.atoms[i].outputs.Disjoint proc.atoms[j].outputs
   := by
+  if hlt : i < j then
+    have ⟨_, _, hatoms, _, _⟩ := haff
+    exact ((List.pairwise_iff_getElem.mp hatoms.2) i j (by simp) (by simp) hlt).2
+  else
+    have ⟨_, _, hatoms, _, _⟩ := haff
+    have hlt : j < i := by omega
+    have := ((List.pairwise_iff_getElem.mp hatoms.2) j i (by simp) (by simp) hlt).2
+    exact this.symm
+
+theorem Proc.AffineChan.getElem_nodup
+  [Arity Op]
+  {proc : Proc Op χ V m n}
+  (haff : proc.AffineChan)
+  (i : Fin proc.atoms.length) :
+    proc.atoms[i].inputs.Nodup ∧ proc.atoms[i].outputs.Nodup
+  := by
   have ⟨_, _, hatoms, _, _⟩ := haff
-  exact (hatoms.2 i j hne).2
+  apply hatoms.1
+  simp
 
 end Wavelet.Dataflow
