wavelet-core/lean/Wavelet/Thm/Seq.lean
@@ -1,3 +1,4 @@
+import Wavelet.Thm.Seq.AffineVar
 import Wavelet.Thm.Seq.Invariants
 import Wavelet.Thm.Seq.Prog
 import Wavelet.Thm.Seq.VarMap
